Changed prefix predicates and prefix lemmas to be indexed by ORDINAL rather than by nat. For the ternary operators ==# and !=#, allow either "nat" or "ORDINAL" as the type of the index argument. Added syntax to switch back to nat (add "[nat]" just before the open parenthesis of the parameter list). Todo: A check is still needed to make sure [nat] and [ORDINAL] are used consistently among mutually recursive components, and there also needs to be a refinement check on this information. Added a few axioms about the combined effect of ORDINAL + and -. Added IsSucc member to type ORDINAL. It returns the negation of IsLimit (in particular, IsSucc is true of 0). Show declaration of _k (and its type) in hover text.

Binaries/DafnyRuntime.cs
@@ -1287,6 +1287,9 @@ namespace Dafny
     public static bool BigOrdinal_IsLimit(BigInteger ord) {
       return ord == 0;
     }
+    public static bool BigOrdinal_IsSucc(BigInteger ord) {
+      return 0 < ord;
+    }
     public static BigInteger BigOrdinal_Offset(BigInteger ord) {
       return ord;
     }
