Source/Dafny/Parser.cs
@@ -1676,6 +1676,7 @@ int StringToInt(string s, int defaultValue, string errString) {
 		IToken signatureEllipsis = null;
 		bool missingOpenParen;
 		bool isTwoState = false;
+		FixpointPredicate.KType kType = FixpointPredicate.KType.Unspecified;
 		
 		if (la.kind == 46) {
 			Get();
@@ -1780,9 +1781,12 @@ int StringToInt(string s, int defaultValue, string errString) {
 				Attribute(ref attrs);
 			}
 			NoUSIdent(out id);
-			if (la.kind == 75 || la.kind == 77 || la.kind == 100) {
+			if (StartOf(11)) {
 				if (la.kind == 77 || la.kind == 100) {
 					GenericParameters(typeArgs, false);
+				}
+				if (la.kind == 73) {
+					KType(ref kType);
 				}
 				Formals(true, isFunctionMethod, false, formals);
 				if (la.kind == 23) {
@@ -1805,9 +1809,12 @@ int StringToInt(string s, int defaultValue, string errString) {
 				Attribute(ref attrs);
 			}
 			NoUSIdent(out id);
-			if (la.kind == 75 || la.kind == 77 || la.kind == 100) {
+			if (StartOf(11)) {
 				if (la.kind == 77 || la.kind == 100) {
 					GenericParameters(typeArgs, false);
+				}
+				if (la.kind == 73) {
+					KType(ref kType);
 				}
 				Formals(true, isFunctionMethod, false, formals);
 				if (la.kind == 23) {
@@ -1820,7 +1827,7 @@ int StringToInt(string s, int defaultValue, string errString) {
 			} else SynErr(182);
 		} else SynErr(183);
 		decreases = isIndPredicate || isCoPredicate ? null : new List<Expression/*!*/>(); 
-		while (StartOf(11)) {
+		while (StartOf(12)) {
 			FunctionSpec(reqs, reads, ens, decreases);
 		}
 		if (la.kind == 71) {
@@ -1842,10 +1849,10 @@ int StringToInt(string s, int defaultValue, string errString) {
 		  f = new Predicate(tok, id.val, dmod.IsStatic, dmod.IsProtected, !isFunctionMethod, typeArgs, formals,
 		                    reqs, reads, ens, new Specification<Expression>(decreases, null), body, Predicate.BodyOriginKind.OriginalOrInherited, attrs, signatureEllipsis);
 		} else if (isIndPredicate) {
-		  f = new InductivePredicate(tok, id.val, dmod.IsStatic, dmod.IsProtected, typeArgs, formals,
+		  f = new InductivePredicate(tok, id.val, dmod.IsStatic, dmod.IsProtected, kType, typeArgs, formals,
 		                             reqs, reads, ens, body, attrs, signatureEllipsis);
 		} else if (isCoPredicate) {
-		  f = new CoPredicate(tok, id.val, dmod.IsStatic, dmod.IsProtected, typeArgs, formals,
+		  f = new CoPredicate(tok, id.val, dmod.IsStatic, dmod.IsProtected, kType, typeArgs, formals,
 		                      reqs, reads, ens, body, attrs, signatureEllipsis);
 		} else {
 		  f = new Function(tok, id.val, dmod.IsStatic, dmod.IsProtected, !isFunctionMethod, typeArgs, formals, result, returnType,
@@ -1887,8 +1894,9 @@ int StringToInt(string s, int defaultValue, string errString) {
 		IToken bodyEnd = Token.NoToken;
 		AllowedDeclModifiers allowed = AllowedDeclModifiers.None;
 		string caption = "";
+		FixpointPredicate.KType kType = FixpointPredicate.KType.Unspecified;
 		
-		while (!(StartOf(12))) {SynErr(184); Get();}
+		while (!(StartOf(13))) {SynErr(184); Get();}
 		switch (la.kind) {
 		case 62: {
 			Get();
@@ -1966,9 +1974,13 @@ int StringToInt(string s, int defaultValue, string errString) {
 		}
 		EncodeExternAsAttribute(dmod, ref attrs, id);
 		
-		if (la.kind == 75 || la.kind == 77 || la.kind == 100) {
+		if (StartOf(11)) {
 			if (la.kind == 77 || la.kind == 100) {
 				GenericParameters(typeArgs, false);
+			}
+			if (la.kind == 73) {
+				KType(ref kType);
+				if (!(isCoLemma || isIndLemma)) { SemErr(t, "type of _k can only be specified for inductive lemmas and co-lemmas"); } 
 			}
 			var isCompilable = (isPlainOlMethod && !dmod.IsGhost) || isConstructor; 
 			Formals(true, isCompilable, isTwoStateLemma, ins);
@@ -1981,7 +1993,7 @@ int StringToInt(string s, int defaultValue, string errString) {
 			Get();
 			signatureEllipsis = t; 
 		} else SynErr(186);
-		while (StartOf(13)) {
+		while (StartOf(14)) {
 			MethodSpec(req, mod, ens, dec, ref decAttrs, ref modAttrs, caption, isConstructor);
 		}
 		if (la.kind == 71) {
@@ -2002,10 +2014,10 @@ int StringToInt(string s, int defaultValue, string errString) {
 		 m = new Constructor(tok, hasName ? id.val : "_ctor", typeArgs, ins,
 		                     req, new Specification<FrameExpression>(mod, modAttrs), ens, new Specification<Expression>(dec, decAttrs), (DividedBlockStmt)body, attrs, signatureEllipsis);
 		} else if (isIndLemma) {
-		 m = new InductiveLemma(tok, id.val, dmod.IsStatic, typeArgs, ins, outs,
+		 m = new InductiveLemma(tok, id.val, dmod.IsStatic, kType, typeArgs, ins, outs,
 		                        req, new Specification<FrameExpression>(mod, modAttrs), ens, new Specification<Expression>(dec, decAttrs), body, attrs, signatureEllipsis);
 		} else if (isCoLemma) {
-		 m = new CoLemma(tok, id.val, dmod.IsStatic, typeArgs, ins, outs,
+		 m = new CoLemma(tok, id.val, dmod.IsStatic, kType, typeArgs, ins, outs,
 		                 req, new Specification<FrameExpression>(mod, modAttrs), ens, new Specification<Expression>(dec, decAttrs), body, attrs, signatureEllipsis);
 		} else if (isLemma) {
 		 m = new Lemma(tok, id.val, dmod.IsStatic, typeArgs, ins, outs,
@@ -2042,7 +2054,7 @@ int StringToInt(string s, int defaultValue, string errString) {
 	void FormalsOptionalIds(List<Formal/*!*/>/*!*/ formals) {
 		Contract.Requires(cce.NonNullElements(formals)); IToken/*!*/ id;  Type/*!*/ ty;  string/*!*/ name;  bool isGhost; 
 		Expect(75);
-		if (StartOf(14)) {
+		if (StartOf(15)) {
 			TypeIdentOptional(out id, out name, out ty, out isGhost);
 			formals.Add(new Formal(id, name, ty, true, isGhost)); 
 			while (la.kind == 24) {
@@ -2447,7 +2459,7 @@ List<MaybeFreeExpression/*!*/>/*!*/ yieldReq, List<MaybeFreeExpression/*!*/>/*!*
 ref Attributes readsAttrs, ref Attributes modAttrs, ref Attributes decrAttrs) {
 		Expression/*!*/ e; FrameExpression/*!*/ fe; bool isFree = false; bool isYield = false; Attributes ensAttrs = null;
 		
-		while (!(StartOf(15))) {SynErr(192); Get();}
+		while (!(StartOf(16))) {SynErr(192); Get();}
 		if (la.kind == 66) {
 			Get();
 			while (IsAttribute()) {
@@ -2474,7 +2486,7 @@ ref Attributes readsAttrs, ref Attributes modAttrs, ref Attributes decrAttrs) {
 				mod.Add(fe); 
 			}
 			OldSemi();
-		} else if (StartOf(16)) {
+		} else if (StartOf(17)) {
 			if (la.kind == 104) {
 				Get();
 				isFree = true;
@@ -2525,7 +2537,7 @@ ref Attributes readsAttrs, ref Attributes modAttrs, ref Attributes decrAttrs) {
 		
 		Expect(71);
 		bodyStart = t; 
-		while (StartOf(17)) {
+		while (StartOf(18)) {
 			Stmt(body);
 		}
 		Expect(72);
@@ -2563,6 +2575,18 @@ ref Attributes readsAttrs, ref Attributes modAttrs, ref Attributes decrAttrs) {
 		} else SynErr(196);
 	}
 
+	void KType(ref FixpointPredicate.KType kType) {
+		Expect(73);
+		if (la.kind == 10) {
+			Get();
+			kType = FixpointPredicate.KType.Nat; 
+		} else if (la.kind == 12) {
+			Get();
+			kType = FixpointPredicate.KType.ORDINAL; 
+		} else SynErr(197);
+		Expect(74);
+	}
+
 	void MethodSpec(List<MaybeFreeExpression> req, List<FrameExpression> mod, List<MaybeFreeExpression> ens,
 List<Expression> decreases, ref Attributes decAttrs, ref Attributes modAttrs, string caption, bool performThisDeprecatedCheck) {
 		Contract.Requires(cce.NonNullElements(req));
@@ -2571,7 +2595,7 @@ List<Expression> decreases, ref Attributes decAttrs, ref Attributes modAttrs, st
 		Contract.Requires(cce.NonNullElements(decreases));
 		Expression e;  FrameExpression fe;  bool isFree = false; Attributes ensAttrs = null;
 		
-		while (!(StartOf(18))) {SynErr(197); Get();}
+		while (!(StartOf(19))) {SynErr(198); Get();}
 		if (la.kind == 65) {
 			Get();
 			while (IsAttribute()) {
@@ -2605,7 +2629,7 @@ List<Expression> decreases, ref Attributes decAttrs, ref Attributes modAttrs, st
 				Expression(out e, false, false);
 				OldSemi();
 				ens.Add(new MaybeFreeExpression(e, isFree, ensAttrs)); 
-			} else SynErr(198);
+			} else SynErr(199);
 		} else if (la.kind == 41) {
 			Get();
 			while (IsAttribute()) {
@@ -2613,7 +2637,7 @@ List<Expression> decreases, ref Attributes decAttrs, ref Attributes modAttrs, st
 			}
 			DecreasesList(decreases, true, false);
 			OldSemi();
-		} else SynErr(199);
+		} else SynErr(200);
 	}
 
 	void DividedBlockStmt(out DividedBlockStmt body, out IToken bodyStart, out IToken bodyEnd) {
@@ -2624,14 +2648,14 @@ List<Expression> decreases, ref Attributes decAttrs, ref Attributes modAttrs, st
 		
 		Expect(71);
 		bodyStart = t; 
-		while (StartOf(17)) {
+		while (StartOf(18)) {
 			Stmt(bodyInit);
 		}
 		if (la.kind == 97) {
 			Get();
 			separatorTok = t; 
 			Expect(31);
-			while (StartOf(17)) {
+			while (StartOf(18)) {
 				Stmt(bodyProper);
 			}
 		}
@@ -2661,7 +2685,7 @@ List<Expression> decreases, ref Attributes decAttrs, ref Attributes modAttrs, st
 			Ident(out id);
 			fieldName = id.val; 
 			fe = new FrameExpression(id, new ImplicitThisExpr(id), fieldName); 
-		} else SynErr(200);
+		} else SynErr(201);
 	}
 
 	void DecreasesList(List<Expression> decreases, bool allowWildcard, bool allowLambda) {
@@ -2719,7 +2743,7 @@ List<Expression> decreases, ref Attributes decAttrs, ref Attributes modAttrs, st
 		Contract.Requires(cce.NonNullElements(reads));
 		Contract.Requires(decreases == null || cce.NonNullElements(decreases));
 		Expression/*!*/ e;  FrameExpression/*!*/ fe; 
-		while (!(StartOf(19))) {SynErr(201); Get();}
+		while (!(StartOf(20))) {SynErr(202); Get();}
 		if (la.kind == 67) {
 			Get();
 			Expression(out e, false, false);
@@ -2749,7 +2773,7 @@ List<Expression> decreases, ref Attributes decAttrs, ref Attributes modAttrs, st
 			
 			DecreasesList(decreases, false, false);
 			OldSemi();
-		} else SynErr(202);
+		} else SynErr(203);
 	}
 
 	void FunctionBody(out Expression/*!*/ e, out IToken bodyStart, out IToken bodyEnd) {
@@ -2766,9 +2790,9 @@ List<Expression> decreases, ref Attributes decAttrs, ref Attributes modAttrs, st
 		if (la.kind == 82) {
 			Get();
 			fe = new FrameExpression(t, new WildcardExpr(t), null); 
-		} else if (StartOf(20)) {
+		} else if (StartOf(21)) {
 			FrameExpression(out fe, allowSemi, false);
-		} else SynErr(203);
+		} else SynErr(204);
 	}
 
 	void PossiblyWildExpression(out Expression e, bool allowLambda) {
@@ -2779,7 +2803,7 @@ List<Expression> decreases, ref Attributes decAttrs, ref Attributes modAttrs, st
 			e = new WildcardExpr(t); 
 		} else if (StartOf(9)) {
 			Expression(out e, false, allowLambda);
-		} else SynErr(204);
+		} else SynErr(205);
 	}
 
 	void Stmt(List<Statement/*!*/>/*!*/ ss) {
@@ -2796,7 +2820,7 @@ List<Expression> decreases, ref Attributes decAttrs, ref Attributes modAttrs, st
 		IToken bodyStart, bodyEnd;
 		int breakCount;
 		
-		while (!(StartOf(21))) {SynErr(205); Get();}
+		while (!(StartOf(22))) {SynErr(206); Get();}
 		switch (la.kind) {
 		case 71: {
 			BlockStmt(out bs, out bodyStart, out bodyEnd);
@@ -2871,8 +2895,8 @@ List<Expression> decreases, ref Attributes decAttrs, ref Attributes modAttrs, st
 					Get();
 					breakCount++; 
 				}
-			} else SynErr(206);
-			while (!(la.kind == 0 || la.kind == 31)) {SynErr(207); Get();}
+			} else SynErr(207);
+			while (!(la.kind == 0 || la.kind == 31)) {SynErr(208); Get();}
 			Expect(31);
 			s = label != null ? new BreakStmt(x, t, label) : new BreakStmt(x, t, breakCount); 
 			break;
@@ -2885,7 +2909,7 @@ List<Expression> decreases, ref Attributes decAttrs, ref Attributes modAttrs, st
 			SkeletonStmt(out s);
 			break;
 		}
-		default: SynErr(208); break;
+		default: SynErr(209); break;
 		}
 	}
 
@@ -2908,12 +2932,12 @@ List<Expression> decreases, ref Attributes decAttrs, ref Attributes modAttrs, st
 				BlockStmt(out proof, out proofStart, out proofEnd);
 			} else if (la.kind == 31) {
 				Get();
-			} else SynErr(209);
+			} else SynErr(210);
 		} else if (la.kind == 84) {
 			Get();
 			dotdotdot = t; 
 			Expect(31);
-		} else SynErr(210);
+		} else SynErr(211);
 		if (dotdotdot != null) {
 		 s = new SkeletonStatement(new AssertStmt(x, t, new LiteralExpr(x, true), null, attrs), dotdotdot, null);
 		} else {
@@ -2937,7 +2961,7 @@ List<Expression> decreases, ref Attributes decAttrs, ref Attributes modAttrs, st
 		} else if (la.kind == 84) {
 			Get();
 			dotdotdot = t; 
-		} else SynErr(211);
+		} else SynErr(212);
 		Expect(31);
 		if (dotdotdot != null) {
 		 s = new SkeletonStatement(new AssumeStmt(x, t, new LiteralExpr(x, true), attrs), dotdotdot, null);
@@ -3018,13 +3042,13 @@ List<Expression> decreases, ref Attributes decAttrs, ref Attributes modAttrs, st
 					suchThatAssume = t; 
 				}
 				Expression(out suchThat, false, true);
-			} else SynErr(212);
+			} else SynErr(213);
 			Expect(31);
 			endTok = t; 
 		} else if (la.kind == 23) {
 			Get();
 			SemErr(t, "invalid statement (did you forget the 'label' keyword?)"); 
-		} else SynErr(213);
+		} else SynErr(214);
 		if (suchThat != null) {
 		 s = new AssignSuchThatStmt(x, endTok, lhss, suchThat, suchThatAssume, null);
 		} else {
@@ -3093,7 +3117,7 @@ List<Expression> decreases, ref Attributes decAttrs, ref Attributes modAttrs, st
 					Expression(out suchThat, false, true);
 				}
 			}
-			while (!(la.kind == 0 || la.kind == 31)) {SynErr(214); Get();}
+			while (!(la.kind == 0 || la.kind == 31)) {SynErr(215); Get();}
 			Expect(31);
 			endTok = t; 
 			ConcreteUpdateStatement update;
@@ -3129,11 +3153,11 @@ List<Expression> decreases, ref Attributes decAttrs, ref Attributes modAttrs, st
 				}
 				Expect(27);
 				SemErr(pat.tok, "LHS of assign-such-that expression must be variables, not general patterns"); 
-			} else SynErr(215);
+			} else SynErr(216);
 			Expression(out e, false, true);
 			Expect(31);
 			s = new LetStmt(e.tok, e.tok, pat, e); 
-		} else SynErr(216);
+		} else SynErr(217);
 	}
 
 	void IfStmt(out Statement/*!*/ ifStmt) {
@@ -3153,11 +3177,11 @@ List<Expression> decreases, ref Attributes decAttrs, ref Attributes modAttrs, st
 		if (IsAlternative()) {
 			AlternativeBlock(true, out alternatives, out usesOptionalBraces, out endTok);
 			ifStmt = new AlternativeStmt(x, endTok, alternatives, usesOptionalBraces); 
-		} else if (StartOf(22)) {
+		} else if (StartOf(23)) {
 			if (IsExistentialGuard()) {
 				ExistentialGuard(out guard, true);
 				isExistentialGuard = true; 
-			} else if (StartOf(23)) {
+			} else if (StartOf(24)) {
 				Guard(out guard);
 			} else {
 				Get();
@@ -3173,7 +3197,7 @@ List<Expression> decreases, ref Attributes decAttrs, ref Attributes modAttrs, st
 				} else if (la.kind == 71) {
 					BlockStmt(out bs, out bodyStart, out bodyEnd);
 					els = bs; endTok = bs.EndTok; 
-				} else SynErr(217);
+				} else SynErr(218);
 			}
 			if (guardEllipsis != null) {
 			 ifStmt = new SkeletonStatement(new IfStmt(x, endTok, isExistentialGuard, guard, thn, els), guardEllipsis, null);
@@ -3181,7 +3205,7 @@ List<Expression> decreases, ref Attributes decAttrs, ref Attributes modAttrs, st
 			 ifStmt = new IfStmt(x, endTok, isExistentialGuard, guard, thn, els);
 			}
 			
-		} else SynErr(218);
+		} else SynErr(219);
 	}
 
 	void WhileStmt(out Statement stmt) {
@@ -3204,20 +3228,20 @@ List<Expression> decreases, ref Attributes decAttrs, ref Attributes modAttrs, st
 		Expect(114);
 		x = t; 
 		if (IsLoopSpec() || IsAlternative()) {
-			while (StartOf(24)) {
+			while (StartOf(25)) {
 				LoopSpec(invariants, decreases, ref mod, ref decAttrs, ref modAttrs);
 			}
 			AlternativeBlock(false, out alternatives, out usesOptionalBraces, out endTok);
 			stmt = new AlternativeLoopStmt(x, endTok, invariants, new Specification<Expression>(decreases, decAttrs), new Specification<FrameExpression>(mod, modAttrs), alternatives, usesOptionalBraces); 
-		} else if (StartOf(22)) {
-			if (StartOf(23)) {
+		} else if (StartOf(23)) {
+			if (StartOf(24)) {
 				Guard(out guard);
 				Contract.Assume(guard == null || cce.Owner.None(guard)); 
 			} else {
 				Get();
 				guardEllipsis = t; 
 			}
-			while (StartOf(24)) {
+			while (StartOf(25)) {
 				LoopSpec(invariants, decreases, ref mod, ref decAttrs, ref modAttrs);
 			}
 			if (la.kind == _lbrace) {
@@ -3226,8 +3250,8 @@ List<Expression> decreases, ref Attributes decAttrs, ref Attributes modAttrs, st
 			} else if (la.kind == _ellipsis) {
 				Expect(84);
 				bodyEllipsis = t; endTok = t; isDirtyLoop = false; 
-			} else if (StartOf(25)) {
-			} else SynErr(219);
+			} else if (StartOf(26)) {
+			} else SynErr(220);
 			if (guardEllipsis != null || bodyEllipsis != null) {
 			 if (mod != null) {
 			   SemErr(mod[0].E.tok, "'modifies' clauses are not allowed on refining loops");
@@ -3245,7 +3269,7 @@ List<Expression> decreases, ref Attributes decAttrs, ref Attributes modAttrs, st
 			 stmt = new WhileStmt(x, endTok, guard, invariants, new Specification<Expression>(decreases, decAttrs), new Specification<FrameExpression>(mod, modAttrs), body);
 			}
 			
-		} else SynErr(220);
+		} else SynErr(221);
 	}
 
 	void MatchStmt(out Statement/*!*/ s) {
@@ -3265,12 +3289,12 @@ List<Expression> decreases, ref Attributes decAttrs, ref Attributes modAttrs, st
 				cases.Add(c); 
 			}
 			Expect(72);
-		} else if (StartOf(25)) {
+		} else if (StartOf(26)) {
 			while (la.kind == _case) {
 				CaseStatement(out c);
 				cases.Add(c); 
 			}
-		} else SynErr(221);
+		} else SynErr(222);
 		s = new MatchStmt(x, t, e, cases, usesOptionalBraces); 
 	}
 
@@ -3295,18 +3319,18 @@ List<Expression> decreases, ref Attributes decAttrs, ref Attributes modAttrs, st
 			x = t;
 			errors.Deprecated(t, "the 'parallel' keyword has been deprecated; the comprehension statement now uses the keyword 'forall' (and the parentheses around the bound variables are now optional)");
 			
-		} else SynErr(222);
+		} else SynErr(223);
 		if (la.kind == _openparen) {
 			Expect(75);
 			if (la.kind == 1) {
 				QuantifierDomain(out bvars, out attrs, out range);
 			}
 			Expect(76);
-		} else if (StartOf(26)) {
+		} else if (StartOf(27)) {
 			if (la.kind == _ident) {
 				QuantifierDomain(out bvars, out attrs, out range);
 			}
-		} else SynErr(223);
+		} else SynErr(224);
 		if (bvars == null) { bvars = new List<BoundVar>(); }
 		if (range == null) { range = new LiteralExpr(x, true); }
 		
@@ -3356,7 +3380,7 @@ List<Expression> decreases, ref Attributes decAttrs, ref Attributes modAttrs, st
 		while (IsAttribute()) {
 			Attribute(ref attrs);
 		}
-		if (StartOf(27)) {
+		if (StartOf(28)) {
 			CalcOp(out opTok, out userSuppliedOp);
 			if (userSuppliedOp.ResultOp(userSuppliedOp) == null) { // guard against non-transitive calcOp (like !=)
 			 SemErr(opTok, "the main operator of a calculation must be transitive");
@@ -3370,7 +3394,7 @@ List<Expression> decreases, ref Attributes decAttrs, ref Attributes modAttrs, st
 			Expression(out e, false, true);
 			lines.Add(e); stepOp = null; danglingOperator = null; 
 			Expect(31);
-			if (StartOf(27)) {
+			if (StartOf(28)) {
 				CalcOp(out opTok, out op);
 				var maybeOp = resOp.ResultOp(op);
 				if (maybeOp == null) {
@@ -3395,7 +3419,7 @@ List<Expression> decreases, ref Attributes decAttrs, ref Attributes modAttrs, st
 				} else if (la.kind == 34) {
 					CalcStmt(out subCalc);
 					hintEnd = subCalc.EndTok; subhints.Add(subCalc); 
-				} else SynErr(224);
+				} else SynErr(225);
 			}
 			var h = new BlockStmt(hintStart, hintEnd, subhints); // if the hint is empty, hintStart is the first token of the next line, but it doesn't matter because the block statement is just used as a container
 			hints.Add(h);
@@ -3426,7 +3450,7 @@ List<Expression> decreases, ref Attributes decAttrs, ref Attributes modAttrs, st
 		while (IsAttribute()) {
 			Attribute(ref attrs);
 		}
-		if (StartOf(20)) {
+		if (StartOf(21)) {
 			FrameExpression(out fe, false, true);
 			mod.Add(fe); 
 			while (la.kind == 24) {
@@ -3437,14 +3461,14 @@ List<Expression> decreases, ref Attributes decAttrs, ref Attributes modAttrs, st
 		} else if (la.kind == 84) {
 			Get();
 			ellipsisToken = t; 
-		} else SynErr(225);
+		} else SynErr(226);
 		if (la.kind == 71) {
 			BlockStmt(out body, out bodyStart, out endTok);
 		} else if (la.kind == 31) {
-			while (!(la.kind == 0 || la.kind == 31)) {SynErr(226); Get();}
+			while (!(la.kind == 0 || la.kind == 31)) {SynErr(227); Get();}
 			Get();
 			endTok = t; 
-		} else SynErr(227);
+		} else SynErr(228);
 		s = new ModifyStmt(tok, endTok, mod, attrs, body);
 		if (ellipsisToken != null) {
 		 s = new SkeletonStatement(s, ellipsisToken, null);
@@ -3464,8 +3488,8 @@ List<Expression> decreases, ref Attributes decAttrs, ref Attributes modAttrs, st
 		} else if (la.kind == 105) {
 			Get();
 			returnTok = t; isYield = true; 
-		} else SynErr(228);
-		if (StartOf(28)) {
+		} else SynErr(229);
+		if (StartOf(29)) {
 			Rhs(out r);
 			rhss = new List<AssignmentRhs>(); rhss.Add(r); 
 			while (la.kind == 24) {
@@ -3548,7 +3572,7 @@ List<Expression> decreases, ref Attributes decAttrs, ref Attributes modAttrs, st
 						Expect(76);
 					}
 				}
-			} else SynErr(229);
+			} else SynErr(230);
 			if (ee != null) {
 			 if (display != null) {
 			   r = new TypeRhs(newToken, ty, ee[0], display);
@@ -3567,7 +3591,7 @@ List<Expression> decreases, ref Attributes decAttrs, ref Attributes modAttrs, st
 		} else if (StartOf(9)) {
 			Expression(out e, false, true);
 			r = new ExprRhs(e); 
-		} else SynErr(230);
+		} else SynErr(231);
 		while (la.kind == 71) {
 			Attribute(ref attrs);
 		}
@@ -3582,13 +3606,13 @@ List<Expression> decreases, ref Attributes decAttrs, ref Attributes modAttrs, st
 			while (la.kind == 29 || la.kind == 73 || la.kind == 75) {
 				Suffix(ref e);
 			}
-		} else if (StartOf(29)) {
+		} else if (StartOf(30)) {
 			ConstAtomExpression(out e, false, false);
 			Suffix(ref e);
 			while (la.kind == 29 || la.kind == 73 || la.kind == 75) {
 				Suffix(ref e);
 			}
-		} else SynErr(231);
+		} else SynErr(232);
 	}
 
 	void NewArray(out List<Expression> ee, out Expression arrayElementInit, out List<Expression> display ) {
@@ -3632,7 +3656,7 @@ List<Expression> decreases, ref Attributes decAttrs, ref Attributes modAttrs, st
 					Expect(74);
 				}
 			}
-		} else SynErr(232);
+		} else SynErr(233);
 		if (ee.Count == 0) {
 		 // an error occurred while parsing, but we still want to make sure to return a nonempty "ee"
 		 ee.Add(new LiteralExpr(x, 0));
@@ -3694,7 +3718,7 @@ List<Expression> decreases, ref Attributes decAttrs, ref Attributes modAttrs, st
 			IdentTypeOptional(out bv);
 			pat = new CasePattern(bv.tok, bv);
 			
-		} else SynErr(233);
+		} else SynErr(234);
 		if (pat == null) {
 		 pat = new CasePattern(t, "_ParseError", new List<CasePattern>());
 		}
@@ -3722,7 +3746,7 @@ List<Expression> decreases, ref Attributes decAttrs, ref Attributes modAttrs, st
 				AlternativeBlockCase(allowExistentialGuards, out alt);
 				alternatives.Add(alt); 
 			}
-		} else SynErr(234);
+		} else SynErr(235);
 		endTok = t; 
 	}
 
@@ -3760,7 +3784,7 @@ List<Expression> decreases, ref Attributes decAttrs, ref Attributes modAttrs, st
 		} else if (StartOf(9)) {
 			Expression(out ee, true, true);
 			e = ee; 
-		} else SynErr(235);
+		} else SynErr(236);
 	}
 
 	void AlternativeBlockCase(bool allowExistentialGuards, out GuardedAlternative alt) {
@@ -3775,13 +3799,13 @@ List<Expression> decreases, ref Attributes decAttrs, ref Attributes modAttrs, st
 			isExistentialGuard = true; 
 		} else if (StartOf(9)) {
 			Expression(out e, true, false);
-		} else SynErr(236);
+		} else SynErr(237);
 		Expect(32);
 		body = new List<Statement>(); 
-		while (!(StartOf(30))) {SynErr(237); Get();}
+		while (!(StartOf(31))) {SynErr(238); Get();}
 		while (IsNotEndOfCase()) {
 			Stmt(body);
-			while (!(StartOf(30))) {SynErr(238); Get();}
+			while (!(StartOf(31))) {SynErr(239); Get();}
 		}
 		alt = new GuardedAlternative(x, isExistentialGuard, e, body); 
 	}
@@ -3791,7 +3815,7 @@ List<Expression> decreases, ref Attributes decAttrs, ref Attributes modAttrs, st
 		bool isFree = false; Attributes attrs = null;
 		
 		if (la.kind == 42 || la.kind == 104) {
-			while (!(la.kind == 0 || la.kind == 42 || la.kind == 104)) {SynErr(239); Get();}
+			while (!(la.kind == 0 || la.kind == 42 || la.kind == 104)) {SynErr(240); Get();}
 			if (la.kind == 104) {
 				Get();
 				isFree = true; errors.Deprecated(t, "the 'free' keyword is soon to be deprecated"); 
@@ -3804,7 +3828,7 @@ List<Expression> decreases, ref Attributes decAttrs, ref Attributes modAttrs, st
 			invariants.Add(new MaybeFreeExpression(e, isFree, attrs)); 
 			OldSemi();
 		} else if (la.kind == 41) {
-			while (!(la.kind == 0 || la.kind == 41)) {SynErr(240); Get();}
+			while (!(la.kind == 0 || la.kind == 41)) {SynErr(241); Get();}
 			Get();
 			while (IsAttribute()) {
 				Attribute(ref decAttrs);
@@ -3812,7 +3836,7 @@ List<Expression> decreases, ref Attributes decAttrs, ref Attributes modAttrs, st
 			DecreasesList(decreases, true, true);
 			OldSemi();
 		} else if (la.kind == 65) {
-			while (!(la.kind == 0 || la.kind == 65)) {SynErr(241); Get();}
+			while (!(la.kind == 0 || la.kind == 65)) {SynErr(242); Get();}
 			Get();
 			mod = mod ?? new List<FrameExpression>(); 
 			while (IsAttribute()) {
@@ -3826,7 +3850,7 @@ List<Expression> decreases, ref Attributes decAttrs, ref Attributes modAttrs, st
 				mod.Add(fe); 
 			}
 			OldSemi();
-		} else SynErr(242);
+		} else SynErr(243);
 	}
 
 	void CaseStatement(out MatchCaseStmt/*!*/ c) {
@@ -3865,12 +3889,12 @@ List<Expression> decreases, ref Attributes decAttrs, ref Attributes modAttrs, st
 				arguments.Add(pat); 
 			}
 			Expect(76);
-		} else SynErr(243);
+		} else SynErr(244);
 		Expect(32);
-		while (!(StartOf(30))) {SynErr(244); Get();}
+		while (!(StartOf(31))) {SynErr(245); Get();}
 		while (IsNotEndOfCase()) {
 			Stmt(body);
-			while (!(StartOf(30))) {SynErr(245); Get();}
+			while (!(StartOf(31))) {SynErr(246); Get();}
 		}
 		c = new MatchCaseStmt(x, name, arguments, body); 
 	}
@@ -3969,7 +3993,7 @@ List<Expression> decreases, ref Attributes decAttrs, ref Attributes modAttrs, st
 			x = t;  binOp = BinaryExpr.Opcode.Exp; 
 			break;
 		}
-		default: SynErr(246); break;
+		default: SynErr(247); break;
 		}
 		if (k == null) {
 		 op = new Microsoft.Dafny.CalcStmt.BinaryCalcOp(binOp);
@@ -3984,7 +4008,7 @@ List<Expression> decreases, ref Attributes decAttrs, ref Attributes modAttrs, st
 			Get();
 		} else if (la.kind == 126) {
 			Get();
-		} else SynErr(247);
+		} else SynErr(248);
 	}
 
 	void ImpliesOp() {
@@ -3992,7 +4016,7 @@ List<Expression> decreases, ref Attributes decAttrs, ref Attributes modAttrs, st
 			Get();
 		} else if (la.kind == 128) {
 			Get();
-		} else SynErr(248);
+		} else SynErr(249);
 	}
 
 	void ExpliesOp() {
@@ -4000,7 +4024,7 @@ List<Expression> decreases, ref Attributes decAttrs, ref Attributes modAttrs, st
 			Get();
 		} else if (la.kind == 130) {
 			Get();
-		} else SynErr(249);
+		} else SynErr(250);
 	}
 
 	void AndOp() {
@@ -4008,7 +4032,7 @@ List<Expression> decreases, ref Attributes decAttrs, ref Attributes modAttrs, st
 			Get();
 		} else if (la.kind == 132) {
 			Get();
-		} else SynErr(250);
+		} else SynErr(251);
 	}
 
 	void OrOp() {
@@ -4016,7 +4040,7 @@ List<Expression> decreases, ref Attributes decAttrs, ref Attributes modAttrs, st
 			Get();
 		} else if (la.kind == 134) {
 			Get();
-		} else SynErr(251);
+		} else SynErr(252);
 	}
 
 	void NegOp() {
@@ -4024,7 +4048,7 @@ List<Expression> decreases, ref Attributes decAttrs, ref Attributes modAttrs, st
 			Get();
 		} else if (la.kind == 136) {
 			Get();
-		} else SynErr(252);
+		} else SynErr(253);
 	}
 
 	void Forall() {
@@ -4032,7 +4056,7 @@ List<Expression> decreases, ref Attributes decAttrs, ref Attributes modAttrs, st
 			Get();
 		} else if (la.kind == 137) {
 			Get();
-		} else SynErr(253);
+		} else SynErr(254);
 	}
 
 	void Exists() {
@@ -4040,7 +4064,7 @@ List<Expression> decreases, ref Attributes decAttrs, ref Attributes modAttrs, st
 			Get();
 		} else if (la.kind == 139) {
 			Get();
-		} else SynErr(254);
+		} else SynErr(255);
 	}
 
 	void QSep() {
@@ -4048,7 +4072,7 @@ List<Expression> decreases, ref Attributes decAttrs, ref Attributes modAttrs, st
 			Get();
 		} else if (la.kind == 28) {
 			Get();
-		} else SynErr(255);
+		} else SynErr(256);
 	}
 
 	void EquivExpression(out Expression e0, bool allowSemi, bool allowLambda, bool allowBitwiseOps) {
@@ -4083,7 +4107,7 @@ List<Expression> decreases, ref Attributes decAttrs, ref Attributes modAttrs, st
 					e0 = new BinaryExpr(x, BinaryExpr.Opcode.Exp, e1, e0); 
 					
 				}
-			} else SynErr(256);
+			} else SynErr(257);
 		}
 	}
 
@@ -4126,7 +4150,7 @@ List<Expression> decreases, ref Attributes decAttrs, ref Attributes modAttrs, st
 			 e0 = new BinaryExpr(x, BinaryExpr.Opcode.Or, new LiteralExpr(x, false), e0);
 			}
 			
-		} else if (StartOf(31)) {
+		} else if (StartOf(32)) {
 			RelationalExpression(out e0, allowSemi, allowLambda, allowBitwiseOps);
 			if (IsAndOp() || IsOrOp()) {
 				if (la.kind == 131 || la.kind == 132) {
@@ -4151,9 +4175,9 @@ List<Expression> decreases, ref Attributes decAttrs, ref Attributes modAttrs, st
 						RelationalExpression(out e1, allowSemi, allowLambda, allowBitwiseOps);
 						e0 = new BinaryExpr(x, BinaryExpr.Opcode.Or, e0, e1); 
 					}
-				} else SynErr(257);
+				} else SynErr(258);
 			}
-		} else SynErr(258);
+		} else SynErr(259);
 	}
 
 	void ImpliesExpression(out Expression e0, bool allowSemi, bool allowLambda, bool allowBitwiseOps) {
@@ -4273,7 +4297,7 @@ List<Expression> decreases, ref Attributes decAttrs, ref Attributes modAttrs, st
 				x = t;  op = BinaryExpr.Opcode.RightShift; 
 				Expect(78);
 				x.val = "<<";  Contract.Assert(t.pos == x.pos + 1); 
-			} else SynErr(259);
+			} else SynErr(260);
 			Term(out e1, allowSemi, allowLambda, allowBitwiseOps);
 			e0 = new BinaryExpr(x, op, e0, e1); 
 		}
@@ -4371,7 +4395,7 @@ List<Expression> decreases, ref Attributes decAttrs, ref Attributes modAttrs, st
 			x = t;  op = BinaryExpr.Opcode.Ge; 
 			break;
 		}
-		default: SynErr(260); break;
+		default: SynErr(261); break;
 		}
 	}
 
@@ -4403,7 +4427,7 @@ List<Expression> decreases, ref Attributes decAttrs, ref Attributes modAttrs, st
 		} else if (la.kind == 102) {
 			Get();
 			x = t;  op = BinaryExpr.Opcode.Sub; 
-		} else SynErr(261);
+		} else SynErr(262);
 	}
 
 	void BitvectorFactor(out Expression e0, bool allowSemi, bool allowLambda, bool allowBitwiseOps) {
@@ -4446,7 +4470,7 @@ List<Expression> decreases, ref Attributes decAttrs, ref Attributes modAttrs, st
 					AsExpression(out e1, allowSemi, allowLambda, allowBitwiseOps);
 					e0 = new BinaryExpr(x, op, e0, e1); 
 				}
-			} else SynErr(262);
+			} else SynErr(263);
 		}
 	}
 
@@ -4461,7 +4485,7 @@ List<Expression> decreases, ref Attributes decAttrs, ref Attributes modAttrs, st
 		} else if (la.kind == 141) {
 			Get();
 			x = t;  op = BinaryExpr.Opcode.Mod; 
-		} else SynErr(263);
+		} else SynErr(264);
 	}
 
 	void AsExpression(out Expression e, bool allowSemi, bool allowLambda, bool allowBitwiseOps) {
@@ -4510,7 +4534,7 @@ List<Expression> decreases, ref Attributes decAttrs, ref Attributes modAttrs, st
 			}
 		} else if (IsLambda(allowLambda)) {
 			LambdaExpression(out e, allowSemi, allowBitwiseOps);
-		} else if (StartOf(32)) {
+		} else if (StartOf(33)) {
 			EndlessExpression(out e, allowSemi, allowLambda, allowBitwiseOps);
 		} else if (la.kind == 1) {
 			NameSegment(out e);
@@ -4527,12 +4551,12 @@ List<Expression> decreases, ref Attributes decAttrs, ref Attributes modAttrs, st
 			while (IsSuffix()) {
 				Suffix(ref e);
 			}
-		} else if (StartOf(29)) {
+		} else if (StartOf(30)) {
 			ConstAtomExpression(out e, allowSemi, allowLambda);
 			while (IsSuffix()) {
 				Suffix(ref e);
 			}
-		} else SynErr(264);
+		} else SynErr(265);
 	}
 
 	void MapDisplayExpr(IToken/*!*/ mapToken, bool finite, out Expression e) {
@@ -4585,14 +4609,14 @@ List<Expression> decreases, ref Attributes decAttrs, ref Attributes modAttrs, st
 					GenericInstantiation(typeArgs);
 				} else if (la.kind == 121) {
 					HashCall(id, out openParen, out typeArgs, out args);
-				} else if (StartOf(33)) {
-				} else SynErr(265);
+				} else if (StartOf(34)) {
+				} else SynErr(266);
 				e = new ExprDotName(id, e, id.val, typeArgs);
 				if (openParen != null) {
 				 e = new ApplySuffix(openParen, e, args);
 				}
 				
-			} else SynErr(266);
+			} else SynErr(267);
 		} else if (la.kind == 73) {
 			Get();
 			x = t; 
@@ -4640,7 +4664,7 @@ List<Expression> decreases, ref Attributes decAttrs, ref Attributes modAttrs, st
 						multipleIndices.Add(ee);
 						
 					}
-				} else SynErr(267);
+				} else SynErr(268);
 			} else if (la.kind == 152) {
 				Get();
 				anyDots = true; 
@@ -4648,7 +4672,7 @@ List<Expression> decreases, ref Attributes decAttrs, ref Attributes modAttrs, st
 					Expression(out ee, true, true);
 					e1 = ee; 
 				}
-			} else SynErr(268);
+			} else SynErr(269);
 			if (multipleIndices != null) {
 			 e = new MultiSelectExpr(x, e, multipleIndices);
 			 // make sure an array class with this dimensionality exists
@@ -4692,7 +4716,7 @@ List<Expression> decreases, ref Attributes decAttrs, ref Attributes modAttrs, st
 			}
 			Expect(76);
 			e = new ApplySuffix(openParen, e, args); 
-		} else SynErr(269);
+		} else SynErr(270);
 	}
 
 	void ISetDisplayExpr(IToken/*!*/ setToken, bool finite, out Expression e) {
@@ -4733,7 +4757,7 @@ List<Expression> decreases, ref Attributes decAttrs, ref Attributes modAttrs, st
 				}
 			}
 			Expect(76);
-		} else SynErr(270);
+		} else SynErr(271);
 		while (la.kind == 66 || la.kind == 67) {
 			if (la.kind == 66) {
 				Get();
@@ -4773,7 +4797,7 @@ List<Expression> decreases, ref Attributes decAttrs, ref Attributes modAttrs, st
 				isExistentialGuard = true; 
 			} else if (StartOf(9)) {
 				Expression(out e, true, true);
-			} else SynErr(271);
+			} else SynErr(272);
 			Expect(36);
 			Expression(out e0, true, true, true);
 			Expect(37);
@@ -4842,7 +4866,7 @@ List<Expression> decreases, ref Attributes decAttrs, ref Attributes modAttrs, st
 			NamedExpr(out e, allowSemi, allowLambda, allowBitwiseOps);
 			break;
 		}
-		default: SynErr(272); break;
+		default: SynErr(273); break;
 		}
 	}
 
@@ -4856,8 +4880,8 @@ List<Expression> decreases, ref Attributes decAttrs, ref Attributes modAttrs, st
 			GenericInstantiation(typeArgs);
 		} else if (la.kind == 121) {
 			HashCall(id, out openParen, out typeArgs, out args);
-		} else if (StartOf(33)) {
-		} else SynErr(273);
+		} else if (StartOf(34)) {
+		} else SynErr(274);
 		e = new NameSegment(id, id.val, typeArgs);
 		if (openParen != null) {
 		 e = new ApplySuffix(openParen, e, args);
@@ -4886,7 +4910,7 @@ List<Expression> decreases, ref Attributes decAttrs, ref Attributes modAttrs, st
 			}
 			e = new SeqDisplayExpr(x, elements); 
 			Expect(74);
-		} else SynErr(274);
+		} else SynErr(275);
 	}
 
 	void MultiSetExpr(out Expression e) {
@@ -4910,7 +4934,7 @@ List<Expression> decreases, ref Attributes decAttrs, ref Attributes modAttrs, st
 			Expression(out e, true, true);
 			e = new MultiSetFormingExpr(x, e); 
 			Expect(76);
-		} else SynErr(275);
+		} else SynErr(276);
 	}
 
 	void ConstAtomExpression(out Expression e, bool allowSemi, bool allowLambda) {
@@ -5031,7 +5055,7 @@ List<Expression> decreases, ref Attributes decAttrs, ref Attributes modAttrs, st
 			ParensExpression(out e, allowSemi, allowLambda);
 			break;
 		}
-		default: SynErr(276); break;
+		default: SynErr(277); break;
 		}
 	}
 
@@ -5060,7 +5084,7 @@ List<Expression> decreases, ref Attributes decAttrs, ref Attributes modAttrs, st
 			 n = BigInteger.Zero;
 			}
 			
-		} else SynErr(277);
+		} else SynErr(278);
 	}
 
 	void Dec(out Basetypes.BigDec d) {
@@ -5155,12 +5179,12 @@ List<Expression> decreases, ref Attributes decAttrs, ref Attributes modAttrs, st
 				cases.Add(c); 
 			}
 			Expect(72);
-		} else if (StartOf(34)) {
+		} else if (StartOf(35)) {
 			while (la.kind == _case) {
 				CaseExpression(out c, allowSemi, allowLambda, allowBitwiseOps);
 				cases.Add(c); 
 			}
-		} else SynErr(278);
+		} else SynErr(279);
 		e = new MatchExpr(x, e, cases, usesOptionalBraces); 
 	}
 
@@ -5178,7 +5202,7 @@ List<Expression> decreases, ref Attributes decAttrs, ref Attributes modAttrs, st
 		} else if (la.kind == 138 || la.kind == 139) {
 			Exists();
 			x = t; 
-		} else SynErr(279);
+		} else SynErr(280);
 		QuantifierDomain(out bvars, out attrs, out range);
 		QSep();
 		Expression(out body, allowSemi, allowLambda);
@@ -5231,7 +5255,7 @@ List<Expression> decreases, ref Attributes decAttrs, ref Attributes modAttrs, st
 			AssumeStmt(out s);
 		} else if (la.kind == 34) {
 			CalcStmt(out s);
-		} else SynErr(280);
+		} else SynErr(281);
 	}
 
 	void LetExpr(out Expression e, bool allowSemi, bool allowLambda, bool allowBitwiseOps) {
@@ -5275,7 +5299,7 @@ List<Expression> decreases, ref Attributes decAttrs, ref Attributes modAttrs, st
 			 }
 			}
 			
-		} else SynErr(281);
+		} else SynErr(282);
 		Expression(out e, false, true);
 		letRHSs.Add(e); 
 		while (la.kind == 24) {
@@ -5337,7 +5361,7 @@ List<Expression> decreases, ref Attributes decAttrs, ref Attributes modAttrs, st
 				arguments.Add(pat); 
 			}
 			Expect(76);
-		} else SynErr(282);
+		} else SynErr(283);
 		Expect(32);
 		Expression(out body, allowSemi, allowLambda, allowBitwiseOps);
 		c = new MatchCaseExpr(x, name, arguments, body); 
@@ -5371,7 +5395,7 @@ List<Expression> decreases, ref Attributes decAttrs, ref Attributes modAttrs, st
 		} else if (la.kind == 2) {
 			Get();
 			id = t; 
-		} else SynErr(283);
+		} else SynErr(284);
 		Expect(96);
 		Expression(out e, true, true);
 	}
@@ -5399,6 +5423,7 @@ List<Expression> decreases, ref Attributes decAttrs, ref Attributes modAttrs, st
 		{_x,_x,_x,_x, _x,_x,_x,_x, _x,_x,_x,_x, _x,_x,_x,_x, _x,_x,_x,_x, _x,_x,_x,_x, _x,_x,_x,_x, _x,_x,_x,_x, _x,_x,_x,_x, _x,_x,_x,_x, _x,_x,_x,_x, _x,_T,_T,_T, _x,_x,_x,_x, _x,_x,_x,_x, _x,_x,_x,_x, _x,_x,_T,_T, _T,_x,_x,_x, _x,_x,_x,_x, _x,_x,_x,_x, _x,_x,_x,_x, _x,_x,_x,_x, _x,_x,_x,_x, _x,_x,_x,_x, _x,_x,_x,_x, _x,_x,_x,_x, _x,_x,_x,_T, _x,_x,_x,_x, _x,_x,_x,_x, _x,_x,_x,_x, _x,_x,_x,_x, _x,_x,_x,_x, _x,_x,_x,_x, _x,_x,_x,_x, _x,_x,_x,_x, _x,_x,_x,_x, _x,_x,_x,_x, _x,_x,_x,_x, _x,_x,_x,_x, _x,_x,_x},
 		{_x,_T,_T,_T, _T,_x,_x,_x, _x,_T,_x,_T, _x,_x,_x,_T, _T,_T,_x,_T, _T,_T,_T,_x, _x,_T,_x,_x, _x,_x,_x,_x, _x,_T,_T,_x, _x,_x,_x,_x, _x,_x,_x,_x, _x,_x,_x,_x, _x,_x,_x,_x, _x,_x,_x,_x, _x,_T,_x,_x, _x,_x,_x,_x, _x,_x,_x,_x, _x,_T,_x,_T, _x,_T,_x,_T, _x,_x,_x,_x, _x,_x,_x,_x, _x,_T,_x,_x, _x,_x,_x,_x, _x,_x,_x,_x, _x,_x,_x,_x, _x,_x,_T,_x, _x,_x,_x,_x, _x,_T,_x,_x, _x,_T,_x,_T, _T,_x,_T,_x, _x,_x,_x,_x, _x,_x,_x,_x, _x,_x,_x,_T, _T,_T,_T,_T, _T,_T,_T,_T, _x,_x,_x,_x, _T,_T,_T,_T, _T,_T,_T,_T, _x,_x,_x},
 		{_T,_x,_x,_x, _x,_x,_x,_x, _x,_x,_x,_x, _x,_x,_x,_x, _x,_x,_x,_x, _x,_x,_x,_T, _x,_x,_x,_x, _x,_x,_x,_x, _x,_x,_x,_x, _x,_x,_x,_x, _x,_T,_x,_T, _T,_T,_T,_T, _T,_T,_T,_T, _T,_T,_T,_T, _T,_T,_T,_T, _T,_T,_T,_T, _T,_x,_T,_T, _T,_T,_x,_T, _T,_x,_x,_T, _x,_T,_x,_x, _x,_x,_x,_x, _x,_x,_x,_T, _T,_T,_x,_x, _x,_x,_x,_x, _x,_x,_x,_x, _T,_x,_x,_T, _x,_x,_x,_x, _x,_x,_x,_x, _x,_x,_x,_x, _x,_x,_x,_x, _x,_x,_x,_x, _x,_x,_x,_x, _x,_x,_x,_x, _x,_x,_x,_x, _x,_x,_x,_x, _x,_x,_x,_x, _x,_x,_x,_x, _x,_x,_x,_x, _x,_x,_x},
+		{_x,_x,_x,_x, _x,_x,_x,_x, _x,_x,_x,_x, _x,_x,_x,_x, _x,_x,_x,_x, _x,_x,_x,_x, _x,_x,_x,_x, _x,_x,_x,_x, _x,_x,_x,_x, _x,_x,_x,_x, _x,_x,_x,_x, _x,_x,_x,_x, _x,_x,_x,_x, _x,_x,_x,_x, _x,_x,_x,_x, _x,_x,_x,_x, _x,_x,_x,_x, _x,_x,_x,_x, _x,_T,_x,_T, _x,_T,_x,_x, _x,_x,_x,_x, _x,_x,_x,_x, _x,_x,_x,_x, _x,_x,_x,_x, _x,_x,_x,_x, _T,_x,_x,_x, _x,_x,_x,_x, _x,_x,_x,_x, _x,_x,_x,_x, _x,_x,_x,_x, _x,_x,_x,_x, _x,_x,_x,_x, _x,_x,_x,_x, _x,_x,_x,_x, _x,_x,_x,_x, _x,_x,_x,_x, _x,_x,_x,_x, _x,_x,_x,_x, _x,_x,_x},
 		{_x,_x,_x,_x, _x,_x,_x,_x, _x,_x,_x,_x, _x,_x,_x,_x, _x,_x,_x,_x, _x,_x,_x,_x, _x,_x,_x,_x, _x,_x,_x,_x, _x,_x,_x,_x, _x,_x,_x,_x, _x,_T,_x,_x, _x,_x,_x,_x, _x,_x,_x,_x, _x,_x,_x,_x, _x,_x,_x,_x, _x,_x,_x,_x, _x,_x,_T,_T, _T,_x,_x,_x, _x,_x,_x,_x, _x,_x,_x,_x, _x,_x,_x,_x, _x,_x,_x,_x, _x,_x,_x,_x, _x,_x,_x,_x, _x,_x,_x,_x, _x,_x,_x,_x, _x,_x,_x,_x, _x,_x,_x,_x, _x,_x,_x,_x, _x,_x,_x,_x, _x,_x,_x,_x, _x,_x,_x,_x, _x,_x,_x,_x, _x,_x,_x,_x, _x,_x,_x,_x, _x,_x,_x,_x, _x,_x,_x,_x, _x,_x,_x,_x, _x,_x,_x},
 		{_T,_x,_x,_x, _x,_x,_x,_x, _x,_x,_x,_x, _x,_x,_x,_x, _x,_x,_x,_x, _x,_x,_x,_x, _x,_x,_x,_x, _x,_x,_x,_x, _x,_x,_x,_x, _x,_x,_x,_x, _x,_x,_x,_x, _x,_T,_T,_T, _x,_x,_x,_x, _x,_x,_x,_x, _x,_x,_x,_x, _x,_x,_T,_T, _T,_x,_x,_x, _x,_x,_x,_x, _x,_x,_x,_x, _x,_x,_x,_x, _x,_x,_x,_x, _x,_x,_x,_x, _x,_x,_x,_x, _x,_x,_x,_x, _x,_x,_x,_x, _x,_x,_x,_T, _x,_x,_x,_x, _x,_x,_x,_x, _x,_x,_x,_x, _x,_x,_x,_x, _x,_x,_x,_x, _x,_x,_x,_x, _x,_x,_x,_x, _x,_x,_x,_x, _x,_x,_x,_x, _x,_x,_x,_x, _x,_x,_x,_x, _x,_x,_x,_x, _x,_x,_x},
 		{_x,_x,_x,_x, _x,_x,_x,_x, _x,_x,_x,_x, _x,_x,_x,_x, _x,_x,_x,_x, _x,_x,_x,_x, _x,_x,_x,_x, _x,_x,_x,_x, _x,_x,_x,_x, _x,_x,_x,_x, _x,_T,_x,_x, _x,_x,_x,_x, _x,_x,_x,_x, _x,_x,_x,_x, _x,_x,_x,_x, _x,_x,_x,_x, _x,_T,_x,_T, _T,_x,_x,_x, _x,_x,_x,_x, _x,_x,_x,_x, _x,_x,_x,_x, _x,_x,_x,_x, _x,_x,_x,_x, _x,_x,_x,_x, _x,_x,_x,_x, _x,_x,_x,_x, _T,_x,_x,_x, _x,_x,_x,_x, _x,_x,_x,_x, _x,_x,_x,_x, _x,_x,_x,_x, _x,_x,_x,_x, _x,_x,_x,_x, _x,_x,_x,_x, _x,_x,_x,_x, _x,_x,_x,_x, _x,_x,_x,_x, _x,_x,_x,_x, _x,_x,_x},
@@ -5647,93 +5672,94 @@ public class Errors {
 			case 194: s = "invalid IteratorSpec"; break;
 			case 195: s = "invalid Variance"; break;
 			case 196: s = "invalid TPCharOption"; break;
-			case 197: s = "this symbol not expected in MethodSpec"; break;
-			case 198: s = "invalid MethodSpec"; break;
+			case 197: s = "invalid KType"; break;
+			case 198: s = "this symbol not expected in MethodSpec"; break;
 			case 199: s = "invalid MethodSpec"; break;
-			case 200: s = "invalid FrameExpression"; break;
-			case 201: s = "this symbol not expected in FunctionSpec"; break;
-			case 202: s = "invalid FunctionSpec"; break;
-			case 203: s = "invalid PossiblyWildFrameExpression"; break;
-			case 204: s = "invalid PossiblyWildExpression"; break;
-			case 205: s = "this symbol not expected in OneStmt"; break;
-			case 206: s = "invalid OneStmt"; break;
-			case 207: s = "this symbol not expected in OneStmt"; break;
-			case 208: s = "invalid OneStmt"; break;
-			case 209: s = "invalid AssertStmt"; break;
+			case 200: s = "invalid MethodSpec"; break;
+			case 201: s = "invalid FrameExpression"; break;
+			case 202: s = "this symbol not expected in FunctionSpec"; break;
+			case 203: s = "invalid FunctionSpec"; break;
+			case 204: s = "invalid PossiblyWildFrameExpression"; break;
+			case 205: s = "invalid PossiblyWildExpression"; break;
+			case 206: s = "this symbol not expected in OneStmt"; break;
+			case 207: s = "invalid OneStmt"; break;
+			case 208: s = "this symbol not expected in OneStmt"; break;
+			case 209: s = "invalid OneStmt"; break;
 			case 210: s = "invalid AssertStmt"; break;
-			case 211: s = "invalid AssumeStmt"; break;
-			case 212: s = "invalid UpdateStmt"; break;
+			case 211: s = "invalid AssertStmt"; break;
+			case 212: s = "invalid AssumeStmt"; break;
 			case 213: s = "invalid UpdateStmt"; break;
-			case 214: s = "this symbol not expected in VarDeclStatement"; break;
-			case 215: s = "invalid VarDeclStatement"; break;
+			case 214: s = "invalid UpdateStmt"; break;
+			case 215: s = "this symbol not expected in VarDeclStatement"; break;
 			case 216: s = "invalid VarDeclStatement"; break;
-			case 217: s = "invalid IfStmt"; break;
+			case 217: s = "invalid VarDeclStatement"; break;
 			case 218: s = "invalid IfStmt"; break;
-			case 219: s = "invalid WhileStmt"; break;
+			case 219: s = "invalid IfStmt"; break;
 			case 220: s = "invalid WhileStmt"; break;
-			case 221: s = "invalid MatchStmt"; break;
-			case 222: s = "invalid ForallStmt"; break;
+			case 221: s = "invalid WhileStmt"; break;
+			case 222: s = "invalid MatchStmt"; break;
 			case 223: s = "invalid ForallStmt"; break;
-			case 224: s = "invalid CalcStmt"; break;
-			case 225: s = "invalid ModifyStmt"; break;
-			case 226: s = "this symbol not expected in ModifyStmt"; break;
-			case 227: s = "invalid ModifyStmt"; break;
-			case 228: s = "invalid ReturnStmt"; break;
-			case 229: s = "invalid Rhs"; break;
+			case 224: s = "invalid ForallStmt"; break;
+			case 225: s = "invalid CalcStmt"; break;
+			case 226: s = "invalid ModifyStmt"; break;
+			case 227: s = "this symbol not expected in ModifyStmt"; break;
+			case 228: s = "invalid ModifyStmt"; break;
+			case 229: s = "invalid ReturnStmt"; break;
 			case 230: s = "invalid Rhs"; break;
-			case 231: s = "invalid Lhs"; break;
-			case 232: s = "invalid NewArray"; break;
-			case 233: s = "invalid CasePattern"; break;
-			case 234: s = "invalid AlternativeBlock"; break;
-			case 235: s = "invalid Guard"; break;
-			case 236: s = "invalid AlternativeBlockCase"; break;
-			case 237: s = "this symbol not expected in AlternativeBlockCase"; break;
+			case 231: s = "invalid Rhs"; break;
+			case 232: s = "invalid Lhs"; break;
+			case 233: s = "invalid NewArray"; break;
+			case 234: s = "invalid CasePattern"; break;
+			case 235: s = "invalid AlternativeBlock"; break;
+			case 236: s = "invalid Guard"; break;
+			case 237: s = "invalid AlternativeBlockCase"; break;
 			case 238: s = "this symbol not expected in AlternativeBlockCase"; break;
-			case 239: s = "this symbol not expected in LoopSpec"; break;
+			case 239: s = "this symbol not expected in AlternativeBlockCase"; break;
 			case 240: s = "this symbol not expected in LoopSpec"; break;
 			case 241: s = "this symbol not expected in LoopSpec"; break;
-			case 242: s = "invalid LoopSpec"; break;
-			case 243: s = "invalid CaseStatement"; break;
-			case 244: s = "this symbol not expected in CaseStatement"; break;
+			case 242: s = "this symbol not expected in LoopSpec"; break;
+			case 243: s = "invalid LoopSpec"; break;
+			case 244: s = "invalid CaseStatement"; break;
 			case 245: s = "this symbol not expected in CaseStatement"; break;
-			case 246: s = "invalid CalcOp"; break;
-			case 247: s = "invalid EquivOp"; break;
-			case 248: s = "invalid ImpliesOp"; break;
-			case 249: s = "invalid ExpliesOp"; break;
-			case 250: s = "invalid AndOp"; break;
-			case 251: s = "invalid OrOp"; break;
-			case 252: s = "invalid NegOp"; break;
-			case 253: s = "invalid Forall"; break;
-			case 254: s = "invalid Exists"; break;
-			case 255: s = "invalid QSep"; break;
-			case 256: s = "invalid ImpliesExpliesExpression"; break;
-			case 257: s = "invalid LogicalExpression"; break;
+			case 246: s = "this symbol not expected in CaseStatement"; break;
+			case 247: s = "invalid CalcOp"; break;
+			case 248: s = "invalid EquivOp"; break;
+			case 249: s = "invalid ImpliesOp"; break;
+			case 250: s = "invalid ExpliesOp"; break;
+			case 251: s = "invalid AndOp"; break;
+			case 252: s = "invalid OrOp"; break;
+			case 253: s = "invalid NegOp"; break;
+			case 254: s = "invalid Forall"; break;
+			case 255: s = "invalid Exists"; break;
+			case 256: s = "invalid QSep"; break;
+			case 257: s = "invalid ImpliesExpliesExpression"; break;
 			case 258: s = "invalid LogicalExpression"; break;
-			case 259: s = "invalid ShiftTerm"; break;
-			case 260: s = "invalid RelOp"; break;
-			case 261: s = "invalid AddOp"; break;
-			case 262: s = "invalid BitvectorFactor"; break;
-			case 263: s = "invalid MulOp"; break;
-			case 264: s = "invalid UnaryExpression"; break;
-			case 265: s = "invalid Suffix"; break;
+			case 259: s = "invalid LogicalExpression"; break;
+			case 260: s = "invalid ShiftTerm"; break;
+			case 261: s = "invalid RelOp"; break;
+			case 262: s = "invalid AddOp"; break;
+			case 263: s = "invalid BitvectorFactor"; break;
+			case 264: s = "invalid MulOp"; break;
+			case 265: s = "invalid UnaryExpression"; break;
 			case 266: s = "invalid Suffix"; break;
 			case 267: s = "invalid Suffix"; break;
 			case 268: s = "invalid Suffix"; break;
 			case 269: s = "invalid Suffix"; break;
-			case 270: s = "invalid LambdaExpression"; break;
-			case 271: s = "invalid EndlessExpression"; break;
+			case 270: s = "invalid Suffix"; break;
+			case 271: s = "invalid LambdaExpression"; break;
 			case 272: s = "invalid EndlessExpression"; break;
-			case 273: s = "invalid NameSegment"; break;
-			case 274: s = "invalid DisplayExpr"; break;
-			case 275: s = "invalid MultiSetExpr"; break;
-			case 276: s = "invalid ConstAtomExpression"; break;
-			case 277: s = "invalid Nat"; break;
-			case 278: s = "invalid MatchExpression"; break;
-			case 279: s = "invalid QuantifierGuts"; break;
-			case 280: s = "invalid StmtInExpr"; break;
-			case 281: s = "invalid LetExpr"; break;
-			case 282: s = "invalid CaseExpression"; break;
-			case 283: s = "invalid MemberBindingUpdate"; break;
+			case 273: s = "invalid EndlessExpression"; break;
+			case 274: s = "invalid NameSegment"; break;
+			case 275: s = "invalid DisplayExpr"; break;
+			case 276: s = "invalid MultiSetExpr"; break;
+			case 277: s = "invalid ConstAtomExpression"; break;
+			case 278: s = "invalid Nat"; break;
+			case 279: s = "invalid MatchExpression"; break;
+			case 280: s = "invalid QuantifierGuts"; break;
+			case 281: s = "invalid StmtInExpr"; break;
+			case 282: s = "invalid LetExpr"; break;
+			case 283: s = "invalid CaseExpression"; break;
+			case 284: s = "invalid MemberBindingUpdate"; break;
 
       default: s = "error " + n; break;
     }
