Test/dafny0/InductivePredicates.dfy
@@ -22,13 +22,17 @@ lemma {:induction false} M'(k: ORDINAL, x: natinf)
   requires Even#[k](x)
   ensures x.N? && x.n % 2 == 0
 {
-  if 0 < k {
+  if k.IsSucc {
     if {
       case x.N? && x.n == 0 =>
         // trivial
       case x.N? && 2 <= x.n && Even#[k-1](N(x.n - 2)) =>
         M'(k-1, N(x.n - 2));
     }
+  } else {
+    assert k.IsLimit;
+    var k' :| k' < k && Even#[k'](x);
+    M'(k', x);
   }
 }
 
@@ -182,3 +186,44 @@ module Alt {
   {
   }
 }
+
+/***********
+ * These are test cases for monotonicity of the the _k parameter.  However, monotonicity
+ * does not appear to be useful in the test suite, and it is possible that the axioms
+ * about monotonicity are expensive performance-wise.  Therefore, the monotonicity axioms
+ * are currently not produced--they are controled by #if WILLING_TO_TAKE_THE_PERFORMANCE_HIT.
+ ***********
+module Monotonicity {
+  inductive predicate P(x: char)
+
+  lemma MonotonicityP(k: ORDINAL, k': ORDINAL, x: char)
+    requires P#[k](x) && k <= k'
+    ensures P#[k'](x)
+  {
+  }
+
+  inductive predicate Q[nat](x: char)
+
+  lemma MonotonicityQ(k: nat, k': nat, x: char)
+    requires Q#[k](x) && k <= k'
+    ensures Q#[k'](x)
+  {
+  }
+
+  copredicate H[nat](x: char)
+
+  lemma MonotonicityH(k: nat, k': nat, x: char)
+    requires H#[k](x) && k' <= k
+    ensures H#[k'](x)
+  {
+  }
+
+  copredicate J(x: char)
+
+  lemma MonotonicityJ(k: ORDINAL, k': ORDINAL, x: char)
+    requires J#[k](x) && k' <= k
+    ensures J#[k'](x)
+  {
+  }
+}
+************/
