Test/dafny0/TypeConversionsCompile.dfy
@@ -73,6 +73,10 @@ method Main()
   x, handful, a0, w := a.Length, a.Length as Handful, a.Length as Abundance, a.Length as bv32;
   print x, " ", handful, " ", a0, " ", w, "\n";
 
+  OrdinalTests();
+}
+
+method OrdinalTests() {
   var ord: ORDINAL := 143;
   var iord := ord as int;
   var oord := iord as ORDINAL;
